\documentclass[12pt]{article}
\usepackage[paperwidth=180cm,paperheight=20cm, margin=5mm]{geometry}

\usepackage{amsmath}
\usepackage{amssymb}
\usepackage{textcomp}
\usepackage{mathpartir}

\renewcommand{\.}{\hskip 0.7pt}
\renewcommand{\d}{\;\vdash\,}
\renewcommand{\r}{\!\.\rightarrow\!}
\DeclareMathOperator{\type}{\,type}
\DeclareMathOperator{\id}{id}
\DeclareMathOperator{\comp}{comp}
\newcommand{\N}{\mathbb{N}}
\DeclareMathOperator{\s}{s}
\DeclareMathOperator{\ind}{ind}
\DeclareMathOperator{\add}{add}
\DeclareMathOperator{\addz}{add-zero}
\DeclareMathOperator{\adds}{add-succ}
\DeclareMathOperator{\proj}{pr}
\DeclareMathOperator{\refl}{refl} 
\DeclareMathOperator{\apply}{ap} 

\begin{document}

$$
\inferrule
{
    \inferrule
    {
      \inferrule
      {\inferrule
        {\inferrule
          {\inferrule{~}{\Gamma \vdash \N \type} \\ \inferrule{\inferrule{~}{\Gamma \d \s : \N \r \N}}{\Gamma, m\!:\!\N \vdash \s(m) : \N}\textup{ev}}
          {\Gamma,\, m\!:\!\N,\, n\!:\!\N \d \s(m) : \N}
          W \\
        \inferrule
          {\inferrule{~}{\Gamma \vdash \N \type} \\ \inferrule{\inferrule{~}{\Gamma \vdash \N \type}}{\Gamma, n\!:\!\N \vdash n\!:\!\N}\delta}
          {\Gamma,\, m\!:\!\N,\, n\!:\!\N \d n\!:\!\N}
          W}
        {\Gamma,\, m : \N,\, n : \N \d (\s(m) + n) : \N}
        \\
      \inferrule
        {\inferrule{\inferrule
          {\inferrule{~}{\Gamma \vdash \N \type} \\ \inferrule{\inferrule{~}{\Gamma \vdash \N \type}}{\Gamma, m\!:\!\N \vdash m\!:\!\N}\delta}
          {\Gamma,\, m\!:\!\N,\, n\!:\!\N \d m\!:\!\N}
          W \\ \inferrule
          {\inferrule{~}{\Gamma \vdash \N \type} \\ \inferrule{\inferrule{~}{\Gamma \vdash \N \type}}{\Gamma, n\!:\!\N \vdash n\!:\!\N}\delta}
          {\Gamma,\, m\!:\!\N,\, n\!:\!\N \d n\!:\!\N}
          W}{\Gamma,\, m\!:\!\N,\, n\!:\!\N \d (m+n) : \N} \\ TODO }
        {\Gamma, m\!:\!\N, n\!:\!\N \vdash \s(m\!+\!n) : \N}
      }
      {\Gamma,\, m : \N,\, n : \N \d (\s(m) + n = \s(m+n)) \type} \\
    \inferrule
      {\inferrule{\inferrule{\inferrule{\inferrule{~}{\Gamma \vdash \N \type}}{\Gamma, m\!:\!\N \vdash m\!:\!\N}\delta}{\Gamma, m\!:\!\N \d m\!+\!\.0 \equiv m : \N}}{\Gamma, m\!:\!\N \d m \equiv m\!+\!\.0 : \N} \\ 
	{\inferrule
        {\inferrule{\inferrule{\inferrule{~}{\Gamma \d \s : \N \r \N}}{\Gamma,\, m\!:\!\N \d \s(m) : \N}\,\textup{ev}}{\Gamma, m\!:\!\N \d \s(m) \equiv \s(m)\!+\!\.0 : \N} \\ \inferrule{\inferrule{\inferrule{~}{\Gamma \d \s : \N \r \N}}{\Gamma,\, m\!:\!\N \d \s(m):\N}\,\textup{ev}}{\Gamma, m\!:\!\N \d \refl_{\s(m)}\!: \s(m) = \s(m)}}
        {\Gamma,\, m : \N \d \refl_{\s(m)} : \s(m) + 0 = \s(m)}
      }
      }
      {\Gamma,\, m : \N \d \refl_{\s(m)} : \s(m) + 0 = \s(m+0)} \\
    \inferrule {\inferrule
      {\inferrule
        {\inferrule
           {\inferrule{\inferrule
          {\inferrule{~}{\Gamma \vdash \N \type} \\ \inferrule{\inferrule{~}{\Gamma \d \s : \N \r \N}}{\Gamma, m\!:\!\N \vdash \s(m) : \N}\textup{ev}}
          {\Gamma,\, m\!:\!\N,\, n\!:\!\N \d \s(m) : \N}
          W \\ \inferrule
          {\inferrule{~}{\Gamma \vdash \N \type} \\ \inferrule{\inferrule{~}{\Gamma \d \s : \N \r \N}}{\Gamma, n\!:\!\N \vdash \s(n) : \N}\textup{ev}}
          {\Gamma,\, m\!:\!\N,\, n\!:\!\N \d \s(n) : \N}
          W}{\Gamma,\, m\!:\!\N,\, n\!:\!\N \d (\s(m)\!+\!\s(n)) : \N} \\ \inferrule{\inferrule
        {\inferrule
          {\inferrule{~}{\Gamma \vdash \N \type} \\ \inferrule{\inferrule{~}{\Gamma \vdash \N \type}}{\Gamma, m\!:\!\N \vdash m\!:\!\N}\delta}
          {\Gamma,\, m\!:\!\N,\, n\!:\!\N \d m\!:\!\N}
          W \\
        \inferrule
          {\inferrule{~}{\Gamma \vdash \N \type} \\ \inferrule{\inferrule{~}{\Gamma \d \s : \N \r \N}}{\Gamma, n\!:\!\N \vdash \s(n) : \N}\textup{ev}}
          {\Gamma,\, m\!:\!\N,\, n\!:\!\N \d \s(n) : \N}
          W}
        {\Gamma,\, m : \N,\, n : \N \d (m + \s(n)) : \N} \\ \inferrule{\inferrule{~}{\Gamma \vdash \N \type} \\ \inferrule{\inferrule{~}{\Gamma \vdash \N \type} \\ \inferrule{\inferrule{~}{\Gamma \d \s : \N \r \N}}{\Gamma,\, r\!:\!\N \d \s(r) : \N}\,\textup{ev}}{\Gamma,\, n\!:\!\N,\, r\!:\!\N \d \s(r) : \N}W}{\Gamma,\, m\!:\!\N,\, n\!:\!\N,\, r\!:\!\N \d \s(r) : \N}W}{\Gamma,\, m\!:\!\N,\, n\!:\!\N \d \s(m\!+\!\s(n)) : \N}S}
           {\Gamma,\, m : \N,\, n : \N \d (\s(m) + \s(n) = \s(m+\s(n))) \type}
         \\ \inferrule
           {\inferrule
             {\inferrule{\inferrule{\inferrule
          {\inferrule{~}{\Gamma \vdash \N \type} \\ \inferrule{\inferrule{~}{\Gamma \vdash \N \type}}{\Gamma, m\!:\!\N \vdash m\!:\!\N}\delta}
          {\Gamma,\, m\!:\!\N,\, n\!:\!\N \d m\!:\!\N}
          W \\ \inferrule
          {\inferrule{~}{\Gamma \vdash \N \type} \\ \inferrule{\inferrule{~}{\Gamma \vdash \N \type}}{\Gamma, n\!:\!\N \vdash n\!:\!\N}\delta}
          {\Gamma,\, m\!:\!\N,\, n\!:\!\N \d n\!:\!\N}
          W}{\Gamma,\, m\!:\!\N,\, n\!:\!\N \d m+\s(n) \equiv \s(m\!+\!n) : \N}}{\Gamma,\, m\!:\!\N,\, n\!:\!\N \d \s(m\!+\!n) \equiv m+\s(n) : \N}}
             {\Gamma, m\!:\!\N, n\!:\!\N, a : \s(m)\!+\!n = \s(m\!+\!n) \d \s(m\!+\!n) \equiv m\!+\!\s(n) : \N}W
           \\ \inferrule
             {\inferrule
               {\inferrule{\inferrule{\inferrule{\inferrule{~}{\Gamma \vdash \N \type} \\ \inferrule{\inferrule{~}{\Gamma \d \s : \N \r \N}}{\Gamma, m\!:\!\N \vdash \s(m) : \N}\textup{ev}}{\Gamma,\, m\!:\!\N,\, n\!:\!\N \d \s(m) : \N}W \\ \inferrule{\inferrule{~}{\Gamma \vdash \N \type} \\ \inferrule{\inferrule{~}{\Gamma \vdash \N \type}}{\Gamma, n\!:\!\N \vdash n\!:\!\N}\delta}{\Gamma,\, m\!:\!\N,\, n\!:\!\N \d n\!:\!\N}W}{\Gamma,\, m\!:\!\N,\, n\!:\!\N \d \s(m) + \s(n) \equiv \s(\s(m) + n) : \N}}{\Gamma,\, m\!:\!\N,\, n\!:\!\N \d \s(\s(m) + n) \equiv \s(m) + \s(n) : \N}}
               {\Gamma, m\!:\!\N, n\!:\!\N, a : \s(m)\!+\!n = \s(m\!+\!n) \d \s(\s(m) + n) \equiv \s(m) + \s(n) : \N}W
             \\ \inferrule
               {\inferrule {\inferrule
        {\inferrule
          {\inferrule{~}{\Gamma \vdash \N \type} \\ \inferrule{\inferrule{~}{\Gamma \d \s : \N \r \N}}{\Gamma, m\!:\!\N \vdash \s(m) : \N}\textup{ev}}
          {\Gamma,\, m\!:\!\N,\, n\!:\!\N \d \s(m) : \N}
          W \\
        \inferrule
          {\inferrule{~}{\Gamma \vdash \N \type} \\ \inferrule{\inferrule{~}{\Gamma \vdash \N \type}}{\Gamma, n\!:\!\N \vdash n\!:\!\N}\delta}
          {\Gamma,\, m\!:\!\N,\, n\!:\!\N \d n\!:\!\N}
          W}{\Gamma,\, m\!:\!\N,\, n\!:\!\N \d (\s(m)\!+\!n)\!: \N} \\ \inferrule {\inferrule{\inferrule{\inferrule
          {\inferrule{~}{\Gamma \vdash \N \type} \\ \inferrule{\inferrule{~}{\Gamma \vdash \N \type}}{\Gamma, m\!:\!\N \vdash m\!:\!\N}\delta}
          {\Gamma,\, m\!:\!\N,\, n\!:\!\N \d m\!:\!\N}
          W \\ \inferrule
          {\inferrule{~}{\Gamma \vdash \N \type} \\ \inferrule{\inferrule{~}{\Gamma \vdash \N \type}}{\Gamma, n\!:\!\N \vdash n\!:\!\N}\delta}
          {\Gamma,\, m\!:\!\N,\, n\!:\!\N \d n\!:\!\N}
          W}{\Gamma,\, m\!:\!\N,\, n\!:\!\N \d (m\!+\!n) : \N} \\ TODO}{\Gamma,\, m\!:\!\N,\, n\!:\!\N \d \s(m\!+\!n) : \N} \\ \inferrule {\inferrule {\inferrule
                 {\inferrule{\inferrule{\inferrule{~}{\Gamma \d \s : \N \r \N}}{\Gamma,\, m\!:\!\N \d \s : \N \r \N}\,W}{\Gamma,\, m\!:\!\N,\, n\!:\!\N \d \s : \N \r \N}\,W}
                 {\Gamma, m\!:\!\N, n\!:\!\N \d \apply_{\s} : \Pi_{(x:\N)} \Pi_{(y:\N)} (x\!=\!y \rightarrow \s(x)\!=\!\s(y))}}
                 {\Gamma, m\!:\!\N, n\!:\!\N,\, x\!:\!\N \d \apply_{\s}(x) : \Pi_{(y:\N)} (x\!=\!y \rightarrow \s(x)\!=\!\s(y))}\textup{ev}}
                 {\Gamma, m\!:\!\N, n\!:\!\N,\, x\!:\!\N,\, y\!:\!\N \d \apply_{\s}(x, y) : x\!=\!y \rightarrow \s(x)\!=\!\s(y)}\textup{ev}}
                 {\Gamma,\, m\!:\!\N,\, n\!:\!\N,\, x\!:\!\N \d \apply_{\s}(x, \s(m\!+\!n)) : x\!=\!\s(m\!+\!n) \rightarrow \s(x)\!=\!\s(\s(m+n))}S}
                 {\Gamma,\, m\!:\!\N,\, n\!:\!\N \d \apply_{\s}(\s(m)\!+\!n, \s(m\!+\!n)) : \s(m)\!+\!n\!=\!\s(m\!+\!n) \rightarrow \s(\s(m)\!+\!n)\!=\!\s(\s(m+n))}S}
                 {\Gamma,\, m\!:\!\N,\, n\!:\!\N,\; a : \s(m) + n = \s(m+n) \;\d\; \apply_{\s}(\s(m)\!+\!n, \s(m\!+\!n))(a) : \s(\s(m) + n) = \s(\s(m+n))}\textup{ev}}
             {\Gamma,\, m : \N,\, n : \N,\; a : \s(m) + n = \s(m+n) \;\d\; \apply_{\s}(\s(m)\!+\!n, \s(m\!+\!n))(a) \::\: \s(m) + \s(n) = \s(\s(m+n))}TODO
           }
           {\Gamma,\, m : \N,\, n : \N,\, a : \s(m) + n = \s(m+n) \;\d\; \apply_{\s}(\s(m)\!+\!n, \s(m\!+\!n))(a) \::\: \s(m) + \s(n) = \s(m+\s(n))}TODO
        }
        {\Gamma,\, m : \N,\, n : \N \;\d\; \lambda a\,.\.\apply_{\s}(\s(m)\!+\!n, \s(m\!+\!n))(a) \::\: \s(m) + n = \s(m+n) \rightarrow \s(m) + \s(n) = \s(m+\s(n))}\lambda
      }{\Gamma,\, m : \N,\, n : \N \;\d\; \apply_{\s}(\s(m)\!+\!n, \s(m\!+\!n)) \::\: \s(m) + n = \s(m+n) \rightarrow \s(m) + \s(n) = \s(m+\s(n))}\eta}
      {\Gamma,\, m : \N \;\d\; \lambda n \.. \apply_{\s}(\s(m)\!+\!n, \s(m\!+\!n)) \::\: \Pi_{(n:\N)} \left( \s(m) + n = \s(m+n) \rightarrow \s(m) + \s(n) = \s(m+\s(n)) \right)}
      \lambda
    }
    {\Gamma,\; m : \N \;\;\d\;\; \ind_\N(\refl_{\s(m)}, \lambda n \.. \apply_{\s}(\s(m)+n, \s(m+n))) \;:\; \Pi_{(n:\N)} (\s(m) + n = \s(m+n))}
    \N\textup{-ind}
  }
{\Gamma \;\;\d\;\; \lambda m \.. \ind_\N(\refl_{\s(m)}, \lambda n \.. \apply_{\s}(\s(m)+n, \s(m+n))) \;:\; \Pi_{(m:\N)} \Pi_{(n:\N)} (\s(m) + n = \s(m+n))}
\lambda
$$


\end{document}